fix things

src/resource_proofs.v
@@ -11,6 +11,7 @@ Require Import Burrow.gmap_utils.
 Require Import Burrow.rollup.
 Require Import Burrow.indexing.
 Require Import Burrow.locations.
+Require Import Burrow.exchange_proof.
 
 Require Import coq_tricks.Deex.
 
@@ -90,7 +91,7 @@ Definition state_inv (state: State M RI) : Prop :=
   match state with
   | StateCon active l =>
        multiset_no_dupes active /\
-       branch_all_total_in_refinement_domain (refinement_of_nat M RI) (as_tree l) active 0
+       valid_totals (refinement_of_nat M RI) (as_tree l) active
   end.
 
 Instance state_valid : Valid (State M RI) :=
@@ -217,7 +218,8 @@ Instance cell_op_proper_right n :
 Instance node_view_proper roi :
     Proper ((≡) ==> (=) ==> (=) ==> impl) (node_view roi). Admitted.
     
-
+Instance valid_totals_proper roi : Proper ((≡) ==> (=) ==> impl) (valid_totals roi).
+  Admitted.
     
 Instance cell_live_proper :
     Proper ((≡) ==> (=)) cell_live. Admitted.
@@ -302,6 +304,7 @@ Proof.
   unfold state_inv in isv. unfold live in isv. destruct b. unfold "⋅" in isv.
   unfold state_op in isv. destruct isv. clear H. rename H0 into isv.
   unfold is_borrow, lmap_is_borrow in isb.
+  unfold valid_totals in isv. destruct_ands. rename H into isv.
   setoid_rewrite <- as_tree_dot in isv.
   setoid_rewrite <- as_tree_dot in isv.
   setoid_rewrite <- as_tree_dot in isv.
@@ -346,31 +349,8 @@ Definition borrow_exchange_cond (ref: Refinement M M) (z m f m' f' : M) :=
       end
   end.
     
-Definition specific_exchange_cond (ref: Refinement M M) (p m f h s m' f' h' s' : M) :=
-  ∃ j mh ,
-  match rel M M ref (dot f p) with
-  | None => True
-  | Some i1 => m_valid (dot m i1) ->
-      dot j s' = f' /\ m' = dot h' mh /\
-      match rel M M ref (dot (dot j s) p) with
-      | None => False
-      | Some i2 => mov (dot m i1) (dot (dot h mh) i2)
-      end
-  end.
-  
 Definition view_exchange_cond (ref: Refinement M M) (view: M -> Prop) (m f h s m' f' h' s' : M) :=
   ∀ p , view p -> specific_exchange_cond ref p m f h s m' f' h' s'.
-  
-Definition specific_flow_cond p i (t t': Branch M) (active: Lifetime) (down up : PathLoc -> M) :=
-  let q := (p, i) in
-  let r := (p, S i) in
-  let s := (p ++ [i], 0) in
-  specific_exchange_cond (refinement_of_nat M RI i)
-      (node_total_minus_live (refinement_of_nat M RI) (node_of_pl t q) active)
-      (down q) (node_live (node_of_pl t q))
-      (down r) (down s)
-      (up q) (node_live (node_of_pl t' q))
-      (up r) (up s).
   
 Definition view_flow_cond p i (b t t': Branch M) (active: Lifetime) (down up : PathLoc -> M) :=
   let q := (p, i) in
@@ -383,18 +363,11 @@ Definition view_flow_cond p i (b t t': Branch M) (active: Lifetime) (down up : P
       (up q) (node_live (node_of_pl t' q))
       (up r) (up s).
       
-Lemma specific_flows_preserve_branch_all_total_in_refinement_domain t t' active
-  (down up : PathLoc -> M)
-  (flow_update : ∀ p i , specific_flow_cond p i t t' active down up)
-  (batird : branch_all_total_in_refinement_domain (refinement_of_nat M RI) t active 0)
-          : branch_all_total_in_refinement_domain (refinement_of_nat M RI) t' active 0.
-Admitted.
-
 Lemma specific_exchange_cond_add_stuff (ref: Refinement M M) (p m f h s m' f' h' s' stuff : M) :
   specific_exchange_cond ref (dot p stuff) m f h s m' f' h' s'
       -> specific_exchange_cond ref p m (dot f stuff) h s m' (dot f' stuff) h' s'.
 Proof. unfold specific_exchange_cond. intro. rewrite <- tpcm_assoc.
-deex. exists (dot j stuff). exists mh.
+deex. exists (dot j stuff). exists l. exists l'.
 rewrite <- tpcm_assoc. assert (dot p stuff = dot stuff p) by (apply tpcm_comm).
 rewrite <- H0. trivial. destruct (rel M M ref (dot f (dot p stuff))); trivial.
 intro. have ab := H H1. destruct_ands; repeat split; trivial.
@@ -412,46 +385,63 @@ Qed.
 Lemma node_live_op (n1 n2 : Node M) : node_live (n1 ⋅ n2) = dot (node_live n1) (node_live n2).
 Admitted.
 
+Global Instance cell_total_minus_live_proper :
+    Proper ((≡) ==> (=) ==> (=)) (cell_total_minus_live). Admitted.
+    
+Lemma cell_total_minus_live_op a b active
+  : cell_total_minus_live (a ⋅ b) active =
+      dot (cell_total_minus_live a active) (cell_total_minus_live b active). Admitted.
+
 Lemma flows_preserve_branch_all_total_in_refinement_domain b t t' active
+  (se: listset PathLoc)
   (down up : PathLoc -> M)
+  (flow_se : ∀ p i , (p, i) ∉ se -> up (p, i) = unit /\ down (p, i) = unit)
   (flow_update : ∀ p i , view_flow_cond p i b t t' active down up)
-  (batird : branch_all_total_in_refinement_domain (refinement_of_nat M RI) (t⋅b) active 0)
-          : branch_all_total_in_refinement_domain (refinement_of_nat M RI) (t'⋅b) active 0.
+  (down_0 : down ([], 0) = unit)
+  (up_0 : up ([], 0) = unit)
+  (reserved_untouched : ∀ pl, cell_total_minus_live (cell_of_pl t pl) active = cell_total_minus_live (cell_of_pl t' pl) active)
+  (batird : valid_totals (refinement_of_nat M RI) (t⋅b) active)
+          : valid_totals (refinement_of_nat M RI) (t'⋅b) active.
 Proof.
   apply specific_flows_preserve_branch_all_total_in_refinement_domain with
-      (t := t⋅b) (down := down) (up := up); trivial.
-  intros.
-  unfold specific_flow_cond. unfold view_flow_cond in flow_update.
-  have flow_update' := flow_update p i. clear flow_update. rename flow_update' into flow_update.
-  unfold view_exchange_cond in flow_update.
-  
-  assert (node_live (node_of_pl (t ⋅ b) (p, i)) =
-      dot (node_live (node_of_pl t (p, i))) (node_live (node_of_pl b (p,i))))
-  by (setoid_rewrite <- node_of_pl_op; apply node_live_op).
-  rewrite H. clear H.
-  
-  assert (node_live (node_of_pl (t' ⋅ b) (p, i)) =
-      dot (node_live (node_of_pl t' (p, i))) (node_live (node_of_pl b (p,i))))
-  by (setoid_rewrite <- node_of_pl_op; apply node_live_op).
-  rewrite H. clear H.
-  
-  (*rewrite tpcm_assoc. rewrite tpcm_assoc.*)
-  
-  apply specific_exchange_cond_add_stuff.
-  
-  apply flow_update. clear flow_update.
-  apply node_view_le2.
-  apply node_view_le with (b := node_of_pl t (p, i)).
-  setoid_rewrite node_op_comm.
-  setoid_rewrite node_of_pl_op.
-  
-  assert (view_sat (node_view (refinement_of_nat M RI) (node_of_pl (t ⋅ b) (p, i)) active)
-    (node_total_minus_live (refinement_of_nat M RI) (node_of_pl (t ⋅ b) (p, i)) active)).
-  - apply node_view_le_total_minus_live with (idx := plend (p,i)).
-    * apply multiset_le_refl.
-    * generalize batird. rewrite forall_equiv_branch_all_total_in_refinement_domain.
-        intro. apply H.
-  - unfold view_sat in H. trivial.
+      (t0 := t⋅b) (down0 := down) (up0 := up) (se0 := se); trivial.
+  - intros.
+    unfold specific_flow_cond. unfold view_flow_cond in flow_update.
+    have flow_update' := flow_update p i. clear flow_update. rename flow_update' into flow_update.
+    unfold view_exchange_cond in flow_update.
+
+    assert (node_live (node_of_pl (t ⋅ b) (p, i)) =
+        dot (node_live (node_of_pl t (p, i))) (node_live (node_of_pl b (p,i))))
+    by (setoid_rewrite <- node_of_pl_op; apply node_live_op).
+    rewrite H. clear H.
+
+    assert (node_live (node_of_pl (t' ⋅ b) (p, i)) =
+        dot (node_live (node_of_pl t' (p, i))) (node_live (node_of_pl b (p,i))))
+    by (setoid_rewrite <- node_of_pl_op; apply node_live_op).
+    rewrite H. clear H.
+
+    (*rewrite tpcm_assoc. rewrite tpcm_assoc.*)
+
+    apply specific_exchange_cond_add_stuff.
+
+    apply flow_update. clear flow_update.
+    apply node_view_le2.
+    apply node_view_le with (b := node_of_pl t (p, i)).
+    setoid_rewrite node_op_comm.
+    setoid_rewrite node_of_pl_op.
+
+    assert (view_sat (node_view (refinement_of_nat M RI) (node_of_pl (t ⋅ b) (p, i)) active)
+      (node_total_minus_live (refinement_of_nat M RI) (node_of_pl (t ⋅ b) (p, i)) active)).
+    + apply node_view_le_total_minus_live with (idx := plend (p,i)).
+      * apply multiset_le_refl.
+      * unfold valid_totals in batird. destruct_ands. rename H into batird.
+        generalize batird. rewrite forall_equiv_branch_all_total_in_refinement_domain.
+          intro. apply H.
+    + unfold view_sat in H. trivial.
+ - intro. setoid_rewrite <- cell_of_pl_op.
+    rewrite cell_total_minus_live_op.
+    rewrite cell_total_minus_live_op.
+    rewrite reserved_untouched. trivial.
 Qed.
 
 Lemma assoc_comm (a b c : Branch M) : (a ⋅ b) ⋅ c ≡ (a ⋅ c) ⋅ b.
@@ -481,6 +471,14 @@ Definition updog (m: M) (gamma: Loc RI) (alpha: nat) (ri: RI) : (PathLoc -> M) :
         else
           unit
       end.
+      
+Definition updog_se (gamma: Loc RI) (alpha: nat) (ri: RI) : listset PathLoc. Admitted.
+
+Lemma updog_se_okay (m: M) (gamma: Loc RI) (alpha: nat) (ri: RI)
+  : ∀ (p : list nat) (i : nat),
+    (p, i) ∉ updog_se gamma alpha ri
+    → updog m gamma alpha ri (p, i) = unit.
+    Admitted.
 
 Lemma updog_eq_m p i alpha ri gamma m
   (is_in : (p, i) ∈ pls_of_loc (ExtLoc alpha ri gamma))
@@ -534,43 +532,45 @@ Lemma view_exchange_cond_of_no_change ref view x y
   : view_exchange_cond ref view x y unit unit x y unit unit.
 Proof. unfold view_exchange_cond. intro.
   deex. unfold specific_exchange_cond.
-  exists y. exists x. rewrite unit_dot. rewrite unit_dot_left.
+  exists y. exists x. exists x. rewrite unit_dot.
   full_generalize (rel M M ref (dot y p)) as t.
-  destruct t; crush.
-  apply reflex.  
+  destruct t; trivial.
+  repeat split; trivial.
+  - rewrite unit_dot. trivial.
+  - rewrite unit_dot. trivial.
+  - apply reflex.
 Qed.
 
 Lemma view_exchange_cond_of_no_change2 ref view x y z w
   : view_exchange_cond ref view x y x y z w z w.
 Proof. unfold view_exchange_cond. intro.
   deex. unfold specific_exchange_cond. intro.
-  exists unit. exists unit.
+  exists unit. exists unit. exists unit.
   repeat (rewrite unit_dot_left). destruct (rel M M ref (dot y p)); trivial.
-  intro. repeat split.
-  - rewrite unit_dot. trivial.
-  - rewrite unit_dot. apply reflex.
+  intro. repeat split. apply reflex.
 Qed.
 
 Lemma specific_exchange_cond_of_whatever ref a x y m
     : specific_exchange_cond ref a x (dot m y) x m unit y unit unit.
 Proof.
-  unfold specific_exchange_cond. exists y. exists unit.
+  unfold specific_exchange_cond. exists y. exists unit. exists unit.
   replace (dot y m) with (dot m y) by (apply tpcm_comm).
   repeat (rewrite unit_dot_left). destruct (rel M M ref (dot (dot m y) a)); trivial.
   intro. repeat split.
   - apply unit_dot.
-  - rewrite unit_dot. apply reflex.
+  - apply reflex.
 Qed.
 
 Lemma specific_exchange_cond_of_whatever2 ref a x y
     : specific_exchange_cond ref a x y x unit unit y unit unit.
 Proof.
-  unfold specific_exchange_cond. exists y. exists unit.
+  unfold specific_exchange_cond. exists y. exists unit. exists unit.
   rewrite unit_dot.
   destruct (rel M M ref (dot y a)); trivial.
   intro. repeat split; trivial.
+  - rewrite unit_dot_left. trivial.
   - rewrite unit_dot. trivial.
-  - rewrite unit_dot. apply reflex.
+  - apply reflex.
 Qed.
 
 Lemma pl_not_in_of_pl_in_extloc pl alpha (ri: RI) gamma
@@ -603,7 +603,7 @@ Proof.
   unfold view_exchange_cond. unfold specific_exchange_cond. unfold borrow_exchange_cond in *.
   unfold lmap_is_borrow in *.
   intro extra. intro.
-  exists f'. exists m'.
+  exists f'. exists m. exists m'.
   assert (tpcm_le z extra).
   - apply isb with (pl := (p,i)); trivial.
   - unfold tpcm_le in H0. deex. rewrite <- H0.
@@ -613,9 +613,14 @@ Proof.
     intro Q.
     have ec2 := ec Q. repeat split.
     + apply unit_dot.
-    + rewrite unit_dot_left. trivial.
+    + rewrite unit_dot. trivial.
+    + rewrite unit_dot. trivial.
     + repeat (rewrite unit_dot). repeat (rewrite unit_dot_left). trivial.
 Qed.
+
+Lemma cell_total_minus_live_cell_of_pl_build_empty (loc: Loc RI) (f:M) pl lt
+  : cell_total_minus_live (cell_of_pl (build loc (CellCon f ∅)) pl) lt = unit.
+  Admitted.
   
 Lemma borrow_exchange b kappa gamma (m f z m' f': M) alpha (ri: RI)
   (isb: is_borrow kappa (ExtLoc alpha ri gamma) z b)
@@ -643,19 +648,22 @@ Proof.
     
     unfold is_borrow in isb.
     
-    assert (exists active_lifetime , active_lifetime = multiset_add kappa l) by (exists (multiset_add kappa l); trivial). deex. rewrite <- H in *. clear H. clear kappa. clear l.
+    full_generalize (multiset_add kappa l) as active_lifetime.
     
     apply flows_preserve_branch_all_total_in_refinement_domain
       with (t := build (ExtLoc alpha ri gamma) (CellCon f ∅) ⋅ build gamma (CellCon m ∅))
+      (se := updog_se gamma alpha ri)
       (down := updog m gamma alpha ri)
-      (up   := updog m' gamma alpha ri); trivial.
-    
-    intros. unfold view_flow_cond.
-    have the_case : Decision ((p, i) ∈ pls_of_loc (ExtLoc alpha ri gamma)) by solve_decision.
-    destruct the_case.
+      (up   := updog m' gamma alpha ri)
+      ; trivial.
+    + intros. split; apply updog_se_okay; trivial.
+
+    + intros. unfold view_flow_cond.
+      have the_case : Decision ((p, i) ∈ pls_of_loc (ExtLoc alpha ri gamma)) by solve_decision.
+      destruct the_case.
     
     (* interesting case: ext location *)
-    + rewrite (updog_eq_m p i); trivial. rewrite (updog_eq_m p i); trivial.
+    * rewrite (updog_eq_m p i); trivial. rewrite (updog_eq_m p i); trivial.
       rewrite (updog_eq_unit1 p i); trivial. rewrite (updog_eq_unit1 p i); trivial.
       rewrite (updog_eq_unit2 p i); trivial. rewrite (updog_eq_unit2 p i); trivial.
       rewrite <- node_of_pl_op. rewrite <- node_of_pl_op.
@@ -673,11 +681,11 @@ Proof.
       repeat (rewrite unit_dot).
       apply (view_exchange_cond_of_borrow_exchange_cond alpha ri gamma z); trivial.
       
-    + have the_case2 : Decision ((p, i) ∈ pls_of_loc gamma) by solve_decision.
+    * have the_case2 : Decision ((p, i) ∈ pls_of_loc gamma) by solve_decision.
       destruct the_case2.
       
       (* semi-interesting case: base location *)
-      * 
+      --
         rewrite <- (updog_other_eq_both p i); trivial.
         rewrite <- (updog_other_eq_both p i); trivial.
         (*rewrite (updog_base_eq_unit1 p i); trivial. rewrite (updog_base_eq_unit1 p i); trivial.
@@ -701,7 +709,7 @@ Proof.
         apply view_exchange_cond_of_no_change2.
 
       (* uninteresting case *)
-      * 
+      --
         rewrite <- (updog_other_eq_both p i); trivial.
         rewrite <- (updog_other_eq_both p i); trivial.
         rewrite updog_other_eq_unit; trivial.
@@ -717,6 +725,10 @@ Proof.
         rewrite build_rest_triv; trivial.
         unfold cell_live, triv_cell. repeat (rewrite unit_dot).
         apply view_exchange_cond_of_no_change2.
+   + setoid_rewrite <- cell_of_pl_op.
+     setoid_rewrite cell_total_minus_live_op.
+     intro.
+     repeat (rewrite cell_total_minus_live_cell_of_pl_build_empty). trivial.
 Qed.
 
 (****************************************************************)
@@ -770,29 +782,31 @@ Proof.
   full_generalize (multiset_add empty_lifetime l) as lt.
   full_generalize (as_tree p) as q. clear p.
   
-  apply specific_flows_preserve_branch_all_total_in_refinement_domain
+  eapply specific_flows_preserve_branch_all_total_in_refinement_domain
     with (t := (build gamma (CellCon m ∅) ⋅ q))
+         (se := updog_se gamma (alloc_alpha (branch_op (build gamma (CellCon m ∅)) q) ri) ri)
          (down := updog m gamma (alloc_alpha (branch_op (build gamma (CellCon m ∅)) q) ri) ri)
          (up   := λ pl, unit); trivial.
-  intros. 
+         
+  - intros. split; trivial. apply updog_se_okay; trivial.
   
-  assert (is_fresh_nat (branch_op (build gamma (CellCon m ∅)) q) (nat_of_extstep (alloc_alpha (branch_op (build gamma (CellCon m ∅)) q) ri) ri)) by (apply is_fresh_alloc; trivial).
-  rename H0 into is_fresh.
-  
-  full_generalize (alloc_alpha (branch_op (build gamma (CellCon m ∅)) q) ri) as alpha.
-  
-  
-  unfold specific_flow_cond.
-  repeat (rewrite unit_dot_left).
-  repeat (rewrite unit_dot).
-   
-  intros.
-  have the_case : Decision ((p, i) ∈ pls_of_loc (ExtLoc alpha ri gamma)) by solve_decision.
-  destruct the_case.
+  - assert (is_fresh_nat (branch_op (build gamma (CellCon m ∅)) q) (nat_of_extstep (alloc_alpha (branch_op (build gamma (CellCon m ∅)) q) ri) ri)) by (apply is_fresh_alloc; trivial).
+    rename H0 into is_fresh.
 
-  (* interesting case: ext location *)
+    full_generalize (alloc_alpha (branch_op (build gamma (CellCon m ∅)) q) ri) as alpha.
+
+
+    unfold specific_flow_cond.
+    repeat (rewrite unit_dot_left).
+    repeat (rewrite unit_dot).
+
+    intros.
+    have the_case : Decision ((p, i) ∈ pls_of_loc (ExtLoc alpha ri gamma)) by solve_decision.
+    destruct the_case.
+
+    (* interesting case: ext location *)
   
-  - rewrite (updog_eq_m p i); trivial. 
+  + rewrite (updog_eq_m p i); trivial. 
     rewrite (updog_eq_unit1 p i); trivial.
     rewrite (updog_eq_unit2 p i); trivial.
     rewrite <- node_of_pl_op. rewrite <- node_of_pl_op.
@@ -823,7 +837,7 @@ Proof.
     repeat (rewrite unit_dot).
     
     unfold specific_exchange_cond.
-    exists f. exists unit.
+    exists f. exists m. exists unit.
     repeat (rewrite unit_dot).
     unfold refinement_of_nat.
     have j := i_value_of_pls_of_loc_ext p i gamma alpha ri e. rewrite j.
@@ -834,11 +848,11 @@ Proof.
     repeat (rewrite unit_dot_left).
     intro. repeat split; trivial. apply reflex.
     
-    - have the_case2 : Decision ((p, i) ∈ pls_of_loc gamma) by solve_decision.
+    + have the_case2 : Decision ((p, i) ∈ pls_of_loc gamma) by solve_decision.
       destruct the_case2.
       
       (* semi-interesting case: base location *)
-      + 
+      * 
         rewrite <- (updog_other_eq_both p i); trivial.
         rewrite (updog_base_eq_m p i); trivial.
         
@@ -854,7 +868,7 @@ Proof.
         apply specific_exchange_cond_of_whatever.
 
       (* uninteresting case *)
-      + 
+      * 
         rewrite <- (updog_other_eq_both p i); trivial.
         rewrite updog_other_eq_unit; trivial.
 
@@ -866,6 +880,10 @@ Proof.
         rewrite build_rest_triv; trivial.
         repeat (rewrite unit_dot_left).
         apply specific_exchange_cond_of_whatever2.
+  - setoid_rewrite <- cell_of_pl_op.
+    setoid_rewrite cell_total_minus_live_op.
+    intro.
+    repeat (rewrite cell_total_minus_live_cell_of_pl_build_empty). trivial.
 Qed.
 
 (****************************************************************)
@@ -876,10 +894,16 @@ Qed.
 
 Definition max_ltunit_in_branch (b: Branch M) : nat. Admitted.
 
-Lemma branch_all_total_in_refinement_domain_of_preserved_cell_totals ref b1 b2 lt1 lt2 idx
+(*Lemma branch_all_total_in_refinement_domain_of_preserved_cell_totals ref b1 b2 lt1 lt2 idx
   (pres: ∀ pl , cell_total (cell_of_pl b1 pl) lt1 = cell_total (cell_of_pl b2 pl) lt2)
   (batird : branch_all_total_in_refinement_domain ref b1 lt1 idx)
   : branch_all_total_in_refinement_domain ref b2 lt2 idx.
+Admitted.*)
+
+Lemma valid_totals_of_preserved_cell_totals ref b1 b2 lt1 lt2
+  (pres: ∀ pl , cell_total (cell_of_pl b1 pl) lt1 = cell_total (cell_of_pl b2 pl) lt2)
+  (batird : valid_totals ref b1 lt1)
+    : valid_totals ref b2 lt2.
 Admitted.
 
 Lemma lt_singleton_not_eq_to_cell_lt ltunit b pl
@@ -929,7 +953,7 @@ Proof.
     rewrite multiset_add_empty_left in H0.
     setoid_rewrite <- as_tree_dot in H0.
     setoid_rewrite as_tree_singleton in H0.
-    apply branch_all_total_in_refinement_domain_of_preserved_cell_totals
+    eapply valid_totals_of_preserved_cell_totals
       with (b1 := build gamma (CellCon m ∅) ⋅ as_tree p)
            (lt1 := active_lifetime); trivial.
     intro.
