src/a.v
@@ -1,0 +1,6 @@
+Require Import Arith.
+
+Lemma stuff (n: nat) (l: list nat)
+  : length l = n -> l = l.
+Proof.
+  induction n as [n IHn] using lt_wf_ind.
